imp/Artifacts/Basic.lean
@@ -1,10 +1,18 @@
 import Aesop
 import Imp
+open Imp
 
-example : {{fun st => st "x" > 0}}(
+example : {{fun st => st "x" > st "y"}}(
 imp {
-  x := x + 1;
+  x := y;
 }
-){{fun st => st "x" > 1}} := by
+){{fun st => st "x" <= st "y"}} := by
 
-sorry
+simp
+intros σ σ' h1 h2
+cases h2 with
+| assign h2_eq =>
+  simp [Env.set]
+  simp [Expr.eval, Env.get] at h2_eq
+  subst h2_eq
+  apply Int.le_refl
