imp/Artifacts/Basic2.lean
@@ -1,0 +1,19 @@
+import Aesop
+import Imp
+open Imp
+
+example : {{fun st => st "x" > st "y"}}(
+imp {
+  while (x > y) {
+    x := x - 1;
+  }
+}
+){{fun st => st "x" <= st "y"}} := by
+apply hoare_consequence
+. apply hoare_while
+  aesop
+. aesop
+. simp; intros σ h
+  have h0 := Truthy.assert_true (expr { y < x })
+  simp [Assertion.iff] at h0
+  simp [Truthy] at h
